PartialOrderTactic/testing.lean
@@ -1,8 +1,11 @@
--- import Mathlib.Tactic.Partiarith
+--import Mathlib.Tactic.Partiarith
 import PartialOrderTactic.Partiarith
 import Lean.Expr
 
 lemma first (a b c: α) [PartialOrder α] (hab : a ≤ b) (hbc : c = b) : a ≤ c := by partiarith
 
 
-example (a b c d e: α) [PartialOrder α] (hab : a ≤ b) (hac : a ≤ c) (hcb : c ≤ b) (hbd : b ≤ d) (hce : c ≤ e) : a ≤ e := by partiarith
+example (a b c d e: α) [PartialOrder α] (hab : a ≤ b) (hac : a ≤ c) (hbc : c = b) (hbd : b ≤ d) (hce : c ≤ e) : a ≤ e := by partiarith
+
+#check OptionT
+#check Lean.logInfo
